coq/JsCorrectness.v
@@ -101,6 +101,18 @@ Ltac findHyp t :=
   | _ => fail "Unable to find an hypothesis for " t
   end.
 
+Ltac rewrite_morph_option :=
+  match goal with
+  | H : appcontext [ morph_option ?d ?f ?x ] |- _ =>
+    let xn := fresh "x" in
+    sets_eq <- xn: x;
+    destruct xn
+  | H : appcontext [ if_some ?op ?f ] |- _ =>
+    let xn := fresh "x" in
+    sets_eq <- xn: op;
+    destruct xn
+  end.
+
 
 (**************************************************************)
 (** General Lemmae *)
@@ -214,7 +226,7 @@ Definition if_regular_lemma (res : result) S0 R0 M :=
     ((res_type R <> restype_normal /\ S = S0 /\ R = R0)
       \/ M S R).
 
-Ltac deal_with_regular_lemma k H if_out :=
+Ltac deal_with_regular_lemma H if_out :=
   let Hnn := fresh "Hnn" in
   let HE := fresh "HE" in
   let HS := fresh "HS" in
@@ -223,14 +235,14 @@ Ltac deal_with_regular_lemma k H if_out :=
   let S' := fresh "S" in
   let R' := fresh "R" in
   lets (S'&R'&HE&[(Hnn&HS&HR)|HM]): if_out (rm H);
-  [k|repeat match goal with
-            | HM : exists x, _ |- _ =>
-              let x := fresh x in destruct HM as [x HM]
-            end; intuit;
-     repeat match goal with
-            | H : result_out (out_ter ?S1 ?R1) = result_out (out_ter ?S0 ?R0) |- _ =>
-              inverts~ H
-            end].
+  [|repeat match goal with
+           | HM : exists x, _ |- _ =>
+             let x := fresh x in destruct HM as [x HM]
+           end; intuit;
+    repeat match goal with
+           | H : result_out (out_ter ?S1 ?R1) = result_out (out_ter ?S0 ?R0) |- _ =>
+             inverts~ H
+           end].
 
 Lemma if_ter_out : forall res K S R,
   if_ter res K = out_ter S R ->
@@ -248,7 +260,7 @@ Lemma if_success_out : forall res K S R,
     R' = res_intro rt rv rl /\
     K S' rv = out_ter S R).
 Proof.
-  introv H. deal_with_regular_lemma ltac:idtac H if_ter_out; substs.
+  introv H. deal_with_regular_lemma H if_ter_out; substs.
    repeat eexists. left~.
    sets_eq t Et: (res_type R0). repeat eexists.
    rewrite~ res_overwrite_value_if_empty_empty in HM.
@@ -262,7 +274,7 @@ Lemma if_value_out : forall res K S R,
     R' = res_intro rt (resvalue_value v) rl /\
     K S' v = out_ter S R).
 Proof.
-  introv H. deal_with_regular_lemma ltac:idtac H if_ter_out; substs.
+  introv H. deal_with_regular_lemma H if_ter_out; substs.
    repeat eexists. left~.
    sets_eq t Et: (res_type R0). repeat eexists.
    rewrite~ res_overwrite_value_if_empty_empty in HM.
@@ -277,7 +289,7 @@ Lemma if_object_out : forall res K S R,
     R' = res_intro rt (resvalue_value (value_object l)) rl /\
     K S' l = out_ter S R).
 Proof.
-  introv H. deal_with_regular_lemma ltac:idtac H if_ter_out; substs.
+  introv H. deal_with_regular_lemma H if_ter_out; substs.
    repeat eexists. left~.
    sets_eq t Et: (res_type R0). repeat eexists.
    rewrite~ res_overwrite_value_if_empty_empty in HM.
@@ -290,7 +302,7 @@ Lemma run_error_correct : forall S C ne S' R',
   run_error S ne = out_ter S' R' ->
   red_expr S C (spec_error ne) (out_ter S' R').
 Proof.
-  introv E. deal_with_regular_lemma ltac:idtac E if_object_out; substs.
+  introv E. deal_with_regular_lemma E if_object_out; substs.
   unfolds build_error. destruct S as [E L [l S]]. simpls. cases_if; tryfalse.
    inverts HE. false~ Hnn.
   unfolds build_error. destruct S as [E L [l' S]]. simpls.
@@ -300,23 +312,73 @@ Proof.
    apply~ red_spec_build_error_1_no_msg.
 Qed.
 
+Lemma object_has_prop_correct : forall S C l x b,
+  object_has_prop S l x = Some b ->
+  red_expr S C (spec_object_has_prop l x) (out_ter S b).
+Admitted. (* TODO (May be painful) *)
+
+Lemma out_error_or_cst_correct : forall S C str ne v S' R',
+  out_error_or_cst S str (ne : native_error) v = out_ter S' R' ->
+  red_expr S C (spec_error_or_cst str ne v) (out_ter S' R').
+Proof.
+  introv E. unfolds in E. cases_if.
+   apply~ red_spec_error_or_cst_true. apply~ run_error_correct.
+   inverts E. apply~ red_spec_error_or_cst_false.
+Qed.
+
+Lemma run_object_method_correct : forall Z (meth : _ -> Z) S l,
+  (exists O, object_binds S l O) ->
+  object_method meth S l (run_object_method meth S l).
+Proof.
+  introv B. unfolds. unfold run_object_method.
+  eexists. splits~. apply pick_spec. apply B.
+Qed.
+
 Lemma object_get_correct : forall runs run_elements,
   runs_type_correct runs run_elements -> forall S0 C0 v x S R,
   object_get runs S0 C0 v x = out_ter S R ->
   red_expr S0 C0 (spec_object_get v x) (out_ter S R).
-Admitted. (* TODO *)
+Proof.
+  introv RC E. destruct v; tryfalse. simpls.
+  apply~ red_spec_object_get. apply run_object_method_correct.
+   skip. (* TODO:  How can we deal with this? *)
+   skip. (* LATER:  There are some arbitrary left there anyway. *)
+Qed.
 
 Lemma prim_value_get_correct : forall runs run_elements,
   runs_type_correct runs run_elements -> forall S0 C0 v x S R,
   prim_value_get runs S0 C0 v x = out_ter S R ->
   red_expr S0 C0 (spec_prim_value_get v x) (out_ter S R).
-Admitted. (* TODO *)
+Proof.
+  introv RC E. deal_with_regular_lemma E if_object_out; substs.
+   skip. (*apply~ red_spec_prim_value_get.*) (* LATER:  There are some arbitrary left there anyway. *)
+   skip. (* LATER:  There are some arbitrary left there anyway. *)
+Qed.
 
 Lemma env_record_get_binding_value_correct : forall runs run_elements,
   runs_type_correct runs run_elements -> forall S0 C0 L x str S R,
   env_record_get_binding_value runs S0 C0 L x str = out_ter S R ->
   red_expr S0 C0 (spec_env_record_get_binding_value L x str) (out_ter S R).
-Admitted. (* TODO *)
+Proof.
+  introv RC E. do 2 unfolds in E.
+  rewrite_morph_option; simpls; tryfalse.
+  rewrite <- Heap.binds_equiv_read_option in EQx0.
+  applys~ red_spec_env_record_get_binding_value EQx0. destruct e.
+   rewrite_morph_option; simpls; tryfalse.
+    rewrite <- Heap.binds_equiv_read_option in EQx1. destruct p.
+    applys~ red_spec_env_record_get_binding_value_1_decl EQx1.
+    repeat cases_if.
+     apply~ out_error_or_cst_correct.
+     inverts E. apply~ red_spec_returns.
+   do 2 unfolds in E. rewrite_morph_option; simpls; tryfalse.
+    forwards OP: object_has_prop_correct EQx1.
+    applys~ red_spec_env_record_get_binding_value_1_object OP.
+    cases_if; subst.
+     apply~ red_spec_env_record_get_binding_value_obj_2_true.
+      applys~ object_get_correct RC.
+     apply~ red_spec_env_record_get_binding_value_2_false.
+      apply~ out_error_or_cst_correct.
+Qed.
 
 Lemma ref_get_value_correct : forall runs run_elements,
   runs_type_correct runs run_elements -> forall S0 C0 rv S R,
@@ -342,18 +404,18 @@ Qed.
 (** Monadic Constructors, Tactics *)
 
 (* Unfold monadic cnstructors.  The continuation is called on all aborting cases. *)
-Ltac if_unmonad_with k :=
+Ltac if_unmonad_with :=
   match goal with
   | H : if_success ?res ?K = result_out ?o' |- _ =>
-    deal_with_regular_lemma k res H if_success_out
+    deal_with_regular_lemma res H if_success_out
   | H : if_value ?res ?K = result_out ?o' |- _ =>
-    deal_with_regular_lemma k res H if_value_out
+    deal_with_regular_lemma res H if_value_out
   | H : if_object ?res ?K = result_out ?o' |- _ =>
-    deal_with_regular_lemma k res H if_object_out
+    deal_with_regular_lemma res H if_object_out
   end.
 
-Ltac unmonad k :=
-  repeat progress (try if_unmonad_with k; try dealing_follows).
+Ltac unmonad :=
+  repeat progress (try if_unmonad_with; try dealing_follows).
 
 
 (**************************************************************)
@@ -463,3 +525,4 @@ Proof.
 
 Qed.
 *)
+
